\documentclass{article}
\usepackage{graphicx} % Required for inserting images
\usepackage{geometry}
\geometry{left=2.5cm,right=2.5cm,top=2.5cm,bottom=2.5cm}
\usepackage{amsfonts,amssymb,graphics,epsfig,verbatim,bm,latexsym,amsmath,url,amsbsy, amsthm}
\usepackage{enumitem}

\renewcommand{\qedsymbol}{$\blacksquare$}
\renewcommand{\qed}{\hfill\blacksquare}


\title{ATE \& Variance Estimators for the Case with Multiple Treatments and Linear Adjustments}
\author{Juri Trifonov}
\date{\today}

\begin{document}

\maketitle

\section{CAR without Clusters}
\subsection*{Notation}

Let us introduce some additional notations besides the notation used in (Juang et al., 2017).
\begin{align}
& N_a := \sum_{i \in[N]} \mathbb I\{A_i = a\},\;\forall a \in \mathcal{A}  \nonumber \\
& N_0 := \sum_{i \in[N]} \mathbb I\{A_i = 0\} \nonumber \\
& I_{\{a,0\}} := \{i \in[N]: A_i = a\} \cup \{i \in[N]: A_i = 0\}, \;\forall a \in \mathcal{A} \nonumber \\
& \hat{\pi}_a(s) := \frac{N_a(s)}{N(s)}, \; \hat{\pi}_0(s) := \frac{N_0(s)}{N(s)},\;\forall a \in \mathcal{A} \; \text{and} \; \forall s \in \mathcal S   \nonumber \\
& \tilde{A}_i = \begin{cases}1\text{, if }A_i = a, \; \forall a \in \mathcal{A} \\ 0\text{, if }A_i = 0.\end{cases} \nonumber
\end{align}

\subsection*{ATE Estimator}

Let us recall the version for a binary treatment case:
\[\hat{\tau} \equiv \frac{1}{N} \sum_{i = 1}^{N} \left[ \frac{A_i (Y_i - \hat{\mu}(1, S_i, X_i))}{\hat{\pi}(S_i)} - \frac{(1 - A_i) (Y_i- \hat{\mu}(0,S_i,X_i))}{1 - \hat{\pi}(S_i)}  + \hat{\mu}(1, S_i, X_i) - \hat{\mu}(0, S_i, X_i)\right].\]

Since in the case with multiple treatments $\hat{\pi}_a(s) + \hat{\pi}_0(s) \neq 1$, we should make the following corrections to the expression. First, instead of $1 - \hat{\pi}(s)$ we should directly use $\hat{\pi}_0 = \frac{n_0(s)}{n(s)}$. Second, instead of a binary treatment variable $A_i$, we shouls use an indicator variable $\tilde{A}_i = \mathbb{I}\{A_i = 1\}$. Thus, the estimator for any treatment $a \in \mathcal A$ (relative to control) becomes:
\[\hat{\tau}_a \equiv \frac{1}{N} \sum_{i=1}^N \left[\frac{\tilde{A}_i (Y_i - \hat{\mu}(a, S_i, X_i))}{\hat{\pi}_a(S_i)} - \frac{(1 - \tilde{A}_i) (Y_i- \hat{\mu}(0,S_i,X_i))}{\hat{\pi}_0(S_i)} + \hat{\mu}(a, S_i, X_i) - \hat{\mu}(0, S_i, X_i)\right],\]
where 
\[\tilde{A}_i = \begin{cases}1\text{, if }A_i = a, \; \forall a \in \mathcal{A} \\ 0\text{, if }A_i = 0.\end{cases}\]

\subsection*{Variance Estimator}

Recall that the expression of the variance estimator for the binary treatment case has the following form:

\begin{align}
	\hat{\sigma}^2 = \frac{1}{N} \sum_{i=1}^N \left[A_i\hat{\Xi}_{1}^2(\mathcal D_i, S_i) + (1- A_i) \hat{\Xi}_{0}^2(\mathcal D_i, S_i) + \hat{\Xi}_2^2(\mathcal D_i, S_i) \right], \nonumber
\end{align}
where 
\begin{align}
	&\hat{\Xi}_{1}(\mathcal D_i, s) = \tilde{\Xi}_{1}(s) - \frac{1}{N_1(s)} \sum_{j \in I_1(s)} \tilde{\Xi}_{1,j}(\mathcal D_i, s) \nonumber, \\
	&\hat{\Xi}_{0}(\mathcal D_i, s) = \tilde{\Xi}_{0}(s) - \frac{1}{N_0(s)} \sum_{j \in I_0(s)} \tilde{\Xi}_{0,j}(\mathcal D_i, s) \nonumber , \\
	& \hat{\Xi}_2 = \left(\frac{1}{N_1(s)} \sum_{j \in I_1(s)} (Y_j - \hat{\tau} A_j) \right) - \left(\frac{1}{N_0(s)} \sum_{j \in I_0(s)} (Y_j - \hat{\tau} A_j)\right) \nonumber \\
	%- \hat{\tau} \left[N_g - \frac{1}{G(s)} \sum_{k \in I(s)} N_k\right] 
	%& \hat{\Xi}_{2}(\mathcal D_g, s) = \left( \frac{1}{G_1(s)} \sum_{j \in I_1(s)} N_j \bar{Y}_j  -  \frac{1}{G_0(s)} \sum_{j \in I_0 (s)} N_j \bar{Y}_j \right) + \hat{\tau} \frac{1}{G} \sum_{g=1}^G N_g, \nonumber \\
	&\tilde{\Xi}_{1}(\mathcal D_i, s) = \left(1 - \frac{1}{\hat{\pi}(s)} \right) \hat{\mu}(1,s,X_i) - \hat{\mu}(0,s,X_i) + \frac{Y_i}{\hat{\pi}(s)}, \nonumber \\
	& \tilde{\Xi}_{0}(\mathcal D_i, s) = \left(\frac{1}{1 - \hat{\pi}(s)} - 1 \right) \hat{\mu}(0,s,X_i) + \hat{\mu}(1,s,X_i) - \frac{Y_i}{1-\hat{\pi}(s)}. \nonumber
\end{align}

Following the same reasoning as for the ATE estimator, we need to make the following corrections to get the expression for the multiple treatments case.

First, notice that we can rewrite $\tilde{\Xi}_{1}(\mathcal D_i, s)$ and $\tilde{\Xi}_{1}(\mathcal D_i, s)$ as follows:
\begin{align}
\tilde{\Xi}_1(\mathcal D_i,s) = \hat{\mu}(1,s,X_i) - \hat{\mu}(0,s,X_i) + \frac{Y_i - \hat{\mu}(1,s,X_i)}{\hat{\pi}(s)}, \nonumber \\
\tilde{\Xi}_0(\mathcal D_i,s) = \hat{\mu}(1,s,X_i) - \hat{\mu}(0,s,X_i) - \frac{Y_i - \hat{\mu}(0,s,X_i)}{1 - \hat{\pi}(s)} \nonumber.
\end{align}
For the same reasoning as before, to generalize these terms for the multiple treatments scenario we need to substitute $\hat{\pi}_a(s)$ and $\hat{\pi}_0(s)$ for $\hat{\pi}(s)$ and $1 - \hat{\pi}(s)$ respectively.

Combining the corrections, we get the following expression of the variance estimator for every treatment $a \in \mathcal A$:
\begin{align}
	\hat{\sigma}_a^2 = \frac{1}{N} \sum_{i=1}^N \left[\tilde{A}_i\hat{\Xi}_{a}^2(\mathcal D_i, S_i) + (1-\tilde{A}_i) \hat{\Xi}_{0}^2(\mathcal D_i, S_i) + \hat{\Xi}_2^2(\mathcal D_i, S_i)\right], \nonumber
\end{align}
where 
\begin{align}
	&\hat{\Xi}_{a}(\mathcal D_i, s) = \tilde{\Xi}_{a}(s) - \frac{1}{N_a(s)} \sum_{j \in I_a(s)} \tilde{\Xi}_{a,j}(\mathcal D_i, s) \nonumber, \\
	&\hat{\Xi}_{0}(\mathcal D_i, s) = \tilde{\Xi}_{0}(s) - \frac{1}{N_0(s)} \sum_{j \in I_0(s)} \tilde{\Xi}_{0,j}(\mathcal D_i, s) \nonumber , \\
	& \hat{\Xi}_2 = \left(\frac{1}{N_a(s)} \sum_{j \in I_a(s)} (Y_j - \hat{\tau}_a \tilde{A}_j) \right) - \left(\frac{1}{N_0(s)} \sum_{j \in I_0(s)} (Y_j - \hat{\tau}_a  \tilde{A}_j)\right), \nonumber \\
	& \tilde{\Xi}_a(\mathcal D_i,s) = \hat{\mu}(a,s,X_i) - \hat{\mu}(0,s,X_i) + \frac{Y_i - \hat{\mu}(a,s,X_i)}{\hat{\pi}_a(s)}, \nonumber \\
& \tilde{\Xi}_0(\mathcal D_i,s) = \hat{\mu}(a,s,X_i) - \hat{\mu}(0,s,X_i) - \frac{Y_i - \hat{\mu}(0,s,X_i)}{\hat{\pi}_0(s)}. \nonumber
	\end{align}

\section{CAR with Clusters}

Using the same reasoning as before, we can generalize the ATE and variance estimators for the case with clusters and multiple treatments as follows.
\subsection*{ATE Estimator}
\begin{align}
\hat{\tau}_a &= \frac{\sum_{g=1}^G \hat{\Xi}_g}{\sum_{g=1}^G N_g}, \nonumber \\
\hat{\Xi}_g &= \frac{\tilde{A}_g \left(N_g\bar{Y}_g - \hat{\mu}(a,S_g,X_g,N_g)\right)}{\hat{\pi}_a(S_g)} - \frac{(1 - \tilde{A}_g) \left(N_g\bar{Y}_g - \hat{\mu}(0,S_g,X_g,N_g)\right)}{\hat{\pi}_0(S_g)}\nonumber \\
 &+ \hat{\mu}(a,S_g,X_g,N_g) - \hat{\mu}(0,S_g,X_g,N_g), \nonumber
\end{align}
where 
\[\tilde{A}_i = \begin{cases}1\text{, if }A_i = a, \; \forall a \in \mathcal{A} \\ 0\text{, if }A_i = 0.\end{cases}\]

\subsection*{Variance Estimator}
\begin{align}
	\hat{\sigma}_a^2 = \frac{\frac{1}{G} \sum_{g=1}^G\left[\tilde{A}_g\hat{\Xi}_{a}^2(\mathcal D_g, S_g) + (1-\tilde{A}_g) \hat{\Xi}_{0}^2(\mathcal D_g, S_g) + \hat{\Xi}_2^2(\mathcal D_g, S_g) \right]}{\left(\frac{1}{G}\sum_{g=1} N_g\right)^2}, \nonumber
\end{align}
where 
\begin{align}
	&\hat{\Xi}_{a}(\mathcal D_g, s) = \tilde{\Xi}_{a}(s) - \frac{1}{G_1(s)} \sum_{j \in I_1(s)} \tilde{\Xi}_{1,j}(s)  - \hat{\tau}_a \left(N_g - \frac{1}{G(s)} \sum_{j \in I(s)} N_j \right)\nonumber, \\
	&\hat{\Xi}_{0}(\mathcal D_g, s) = \tilde{\Xi}_{0}(s) - \frac{1}{G_0(s)} \sum_{j \in I_0(s)} \tilde{\Xi}_{0,j}(s)  - \hat{\tau}_a \left(N_g - \frac{1}{G(s)} \sum_{j \in I(s)} N_j \right)\nonumber , \\
	& \hat{\Xi}_2(s) = \left(\frac{1}{G_1(s)} \sum_{j \in I_1(s)} N_j \bar{Y}_j\right) - \left(\frac{1}{G_0(s)} \sum_{j \in I_0(s)} N_j \bar{Y}_j\right) - \hat{\tau}_a \times \left(\frac{1}{G(s)}\sum_{j \in I(s)} N_j \right), \nonumber \\
	%- \hat{\tau} \left[N_g - \frac{1}{G(s)} \sum_{k \in I(s)} N_k\right] 
	%& \hat{\Xi}_{2}(\mathcal D_g, s) = \left( \frac{1}{G_1(s)} \sum_{j \in I_1(s)} N_j \bar{Y}_j  -  \frac{1}{G_0(s)} \sum_{j \in I_0 (s)} N_j \bar{Y}_j \right) + \hat{\tau} \frac{1}{G} \sum_{g=1}^G N_g, \nonumber \\
	&\tilde{\Xi}_{a}(\mathcal D_g, s) = \hat{\mu}(a,s,X_g,N_g) - \hat{\mu}(0,s,X_g,N_g) + \frac{N_g \bar{Y}_g - \hat{\mu}(a,s,X_g,N_g)}{\hat{\pi}_a(s)}, \nonumber \\
	& \tilde{\Xi}_{0}(\mathcal D_g, s) = \hat{\mu}(a,s,X_g,N_g) - \hat{\mu}(0,s,X_g,N_g) - \frac{N_g \bar{Y}_g - \hat{\mu}(0,s,X_g,N_g)}{\hat{\pi}_0(s)}. \nonumber
	\end{align}


\end{document}

